coq: ZF: Set.Eval.EvalWhenFunctional

coq/ZF/Set/Eval.v
@@ -2,12 +2,30 @@ Declare Scope ZF_Set_Eval_scope.
 Open    Scope ZF_Set_Eval_scope.
 
 Require Import ZF.Class.
+Require Import ZF.Class.Domain.
 Require Import ZF.Class.Eval.
+Require Import ZF.Class.Functional.
+Require Import ZF.Core.Equiv.
 Require Import ZF.Set.
 Require Import ZF.Set.FromClass.
+Require Import ZF.Set.OrdPair.
 
-Definition eval (P:Class) (a:U) : U := fromClass (Class.Eval.eval P a)
-  (EvalIsSmall P a).
+Definition eval (F:Class) (a:U) : U := fromClass (Class.Eval.eval F a)
+  (EvalIsSmall F a).
 
-Notation "P :( a ):" := (eval P a)
+Notation "F ! a" := (eval F a)
   (at level 0, no associativity) : ZF_Set_Eval_scope.
+
+Proposition EvalWhenFunctional : forall (F:Class) (a y:U),
+  Functional F -> domain F a -> F :(a,y): <-> F!a = y.
+Proof.
+  intros F a y H1 H2. split; intros H3.
+  - apply SameClassEqual. unfold eval.
+    apply ClassEquivTran with (Class.Eval.eval F a).
+    + apply ToClassFromClass.
+    + apply Class.Eval.EvalWhenFunctional; assumption.
+  - apply Class.Eval.EvalWhenFunctional.
+    + assumption.
+    + assumption.
+    + rewrite <- H3. unfold eval. apply ClassEquivSym, ToClassFromClass.
+Qed.
