coq/ZF/Class/FunctionOn.v
@@ -87,7 +87,7 @@ Proposition FunctionOnEquivCharac : forall (F A G B:Class),
   FunctionOn F A ->
   FunctionOn G B ->
   F :~: G       <->
-  A :~: B /\ forall x, A x -> F:(x): = G:(x):.
+  A :~: B /\ forall x, A x -> F!x = G!x.
 Proof.
   intros F A G B [[H1 H2] H3] [[H4 H5] H6]. split; intros H7.
   - split.
